WIP: createEff_consumeEff rewrite

EffectSSA/Rewrites/Convert.lean
@@ -1,5 +1,6 @@
 import EffectSSA.Syntax
 import EffectSSA.Semantics
+import EffectSSA.Rewrites.Basic
 
 /-!
 # Implicit to EffectSSA conversion rewrites
@@ -8,4 +9,24 @@ namespace EffectSSA
 namespace Rewrites
 variable {τ}
 
--- theorem exec_createEff_consumeEff_eq :
+def createEff_consumeEff : Rewrite τ 0 where
+  src := {
+    program := program!()
+    returnVars := []
+  }
+  tgt := {
+    program := program!(
+      e := createEff;
+      consumeEff(e)
+    )
+    returnVars := []
+  }
+
+namespace createEff_consumeEff
+
+theorem welltyped : (@createEff_consumeEff τ).WellFormed ∅ := by
+  use []
+  unfold createEff_consumeEff
+  decide
+
+end createEff_consumeEff
